Protocol/ServiceProvider.fst
@@ -2,9 +2,9 @@ module Serviceprovider
 open Protocol
 
 val serviceprovider:  me:prin -> pubkey me -> privkey me ->
-                      client:prin -> idp:prin -> pubkey idp -> unit 
-let serviceprovider me pubk privk client idp pubkidp = 
-  let reqRes = recieve client in (*1*)
+                      browser:prin -> idp:prin -> pubkey idp -> unit 
+let serviceprovider me pubk privk browser idp pubkidp = 
+  let reqRes = recieve browser in (*1*)
   match reqRes with
   | HttpGet (uri) -> 
   
@@ -12,19 +12,19 @@ let serviceprovider me pubk privk client idp pubkidp =
     assume(Log me authnReq) (*Protocol event*);
     let sigSP = sign me privk authnReq in
       
-    let authnReqest = SamlProtocolMessage idp authnReq sigSP uri in 
-    send client authnReqest; (*2*)  
-    let authResponse = recieve client in (*7*)
+    let authnReqest = SamlProtocolMessage idp authnReq sigSP in 
+    send browser authnReqest; (*2*)  
+    let authResponse = recieve browser in (*7*)
     match authResponse with
-    | SamlProtocolMessage (sp, message, sigIDP, relay) -> 
-      (if verify idp pubkidp message sigIDP
+    | SamlProtocolMessage (sp, msg, sigIDP) -> 
+      (if verify idp pubkidp msg sigIDP
       then
-        ((*assert(Log idp message);*)
+        (assert(Log idp msg);
           let resource = Resource uri in
-          send client resource)  (*8*)
+          send browser resource)  (*8*)
       else ())
-    | _ ->  send client (Failed (403))(*8.1*)     
+    | _ ->  send browser (Failed (403))(*8.1*)     
   
-  | _ -> send client (Failed (400))(*2.1*)
+  | _ -> send browser (Failed (400))(*2.1*)
 
 end (* Serviceprovider *)
