Protocol/identityprovider.fst
@@ -1,22 +1,23 @@
 module Identityprovider
 open Protocol
 
-val identityprovider: me:prin -> pubkey me -> privkey me ->
-                      client:prin -> sp:prin -> pubkey sp -> unit
-let identityprovider me pubk privk client serviceprovider pubksp =
+val identityprovider: me:prin -> pubkey me -> privkey me 
+                      -> browser:prin -> sp:prin -> pubkey sp
+                      -> unit
+let identityprovider me pubk privk browser serviceprovider pubksp =
 	
-  let authRequest = recieve client in (*3*)
-	match authRequest with
-	| SamlProtocolMessage (idp, message, sigSP, relay)->  
+  let samlreq = recieve browser in (*3*)
+	match samlreq with
+	| SamlProtocolMessage (idp, msg, sigSP)->  
 
-    if verify serviceprovider pubksp message sigSP
+    if verify serviceprovider pubksp msg sigSP
     then
-     ( (*assert (Log serviceprovider message);*)
-        let challenge = createChallenge client in
+     (assert (Log serviceprovider msg);
+        let challenge = createChallenge browser in
     
         let challengeMessage = ChallengeMessage challenge in
-        send client challengeMessage; (*4*)
-        let credentials = recieve client in (*5*)
+        send browser challengeMessage; (*4*)
+        let credentials = recieve browser in (*5*)
         match credentials with
           | Credentials(user, password, challenge') -> 
   
@@ -25,14 +26,14 @@ let identityprovider me pubk privk client serviceprovider pubksp =
           let samlresponse = createSamlResponse me serviceprovider Success in
           assume(Log me samlresponse);
           let sigIDP = sign me privk samlresponse in 
-          let response = SamlProtocolMessage serviceprovider samlresponse sigIDP relay in
-          send client response(*6*)
+          let response = SamlProtocolMessage serviceprovider samlresponse sigIDP in
+          send browser response(*6*)
   
-        | _ -> send client (Failed (400)))(*6.3*)
-    else send client (Failed (400))
+        | _ -> send browser (Failed (400)))(*6.3*)
+    else send browser (Failed (400))
   | _ -> 
      let samlresponse = createSamlResponse me serviceprovider Requester in
      assume(Log me samlresponse);
      let sigIDP = sign me privk samlresponse in
-     let response = SamlProtocolMessage serviceprovider samlresponse sigIDP "" in
-     send client response (*4.1*)
+     let response = SamlProtocolMessage serviceprovider samlresponse sigIDP in
+     send browser response (*4.1*)
