Protocol/basic-example.fst
@@ -1,0 +1,108 @@
+module CRYPTO
+type prin = string
+type pubkey :: prin => *
+type privkey :: prin => *
+type dsig 
+
+val keygen:  p:prin
+          -> (pubkey p * privkey p)
+
+type samlmessage =
+  | AuthnRequest: samlmessage
+  | Response: samlmessage
+
+type message =
+  | SamlProtocolMessage: prin -> samlmessage -> dsig -> message
+  | Failed: int -> message
+
+type Says :: prin => samlmessage => E
+
+val sign:  p:prin
+        -> privkey p
+        -> msg:samlmessage{Says p msg}
+        -> dsig
+
+val verify: p:prin
+        -> pubkey p 
+        -> msg:samlmessage
+        -> dsig
+        -> b:bool{b=true ==> Says p msg}
+
+end(* crypto *)
+
+module UTIL
+open CRYPTO
+
+val send: prin -> message -> unit
+val recieve: prin -> message 
+
+val createRequest: prin -> samlmessage
+val createResponse: prin -> samlmessage
+
+val fork: list (unit -> unit) -> unit
+
+(* val send: prin -> (samlmessage * dsig) -> unit
+val recv: prin -> (samlmessage * dsig) 
+val string2bytes: string -> samlmessage*)
+
+end(* util *)
+
+module Serviceprovider
+open CRYPTO
+open UTIL
+val serviceprovider: me:prin -> pubkey me -> privkey me 
+         -> idp:prin -> pubkey idp -> unit
+let serviceprovider me mypk mysk idp serverpk = 
+   let req = createRequest idp in 
+    assume (Says me req); (* protocol event *)
+    let dsig = sign me mysk req in 
+      let authreq = SamlProtocolMessage idp req dsig in
+      send idp authreq;
+      let samlresp = recieve idp in 
+      match samlresp with
+      | SamlProtocolMessage (me', resp, dsig') -> 
+        if verify idp serverpk resp dsig'
+        then (assert (Says idp resp); ())
+        else ()
+      | _ -> ()
+
+end(* Serviceprovider *)
+
+module Identityprovider
+open CRYPTO
+open UTIL
+
+val identityprovider: me:prin -> pubkey me -> privkey me 
+                      -> browser:prin -> sp:prin -> pubkey sp
+                      -> unit
+let identityprovider me pubk privk browser serviceprovider pubksp =
+ 
+   let samlreq = recieve serviceprovider in 
+   match samlreq with
+   | SamlProtocolMessage (me', message, dsig) -> 
+ 
+    if verify serviceprovider pubksp message dsig
+     then 
+       (assert (Says serviceprovider message);
+        let resp = createResponse serviceprovider in 
+        assume (Says me resp);
+        let dsig = sign me privk resp in 
+        let samlresp = SamlProtocolMessage serviceprovider resp dsig in
+        send serviceprovider samlresp)
+     else ()
+   | _ -> ()
+   
+
+end(* identityprovider *)
+
+module MAIN
+open CRYPTO
+open UTIL
+open Serviceprovider
+open Identityprovider
+let main attacker =
+  let sppk, spsk = keygen "serviceprovider" in 
+  let idppk, idpsk = keygen "identityprovider" in 
+  fork [attacker;
+        (fun () -> serviceprovider "serviceprovider" sppk spsk "identityprovider" idppk);
+        (fun () -> identityprovider "identityprovider" idppk idpsk "browser" "serviceprovider" sppk)]
