setenv.sh
@@ -1,5 +1,5 @@
 #!/bin/bash 
 
-PWD="c:\utils\fstar"
+PWD="C:\Utils\FStar\fstar-0.6-alpha"
 export FSTAR_HOME=`cygpath -d "$PWD"`
 export PATH=`cygpath -d "$PWD/bin"`:$PATH
